\documentclass[a4paper,12pt,twoside]{article}

\usepackage{preamble}

\title{Homework 01}
\author{Brandon Henke\\PHY851\\Scott Pratt}
\date{September 9, 2021}

\setcounter{section}{1}

\fancyhead[LE,RO]{B. Henke}
\fancyhead[RE,LO]{\thepage}

\begin{document}
%\tableofcontents

\maketitle
% \begin{multicols*}{2}


\subsection{}%1
\subsubsection*{a}
\begin{align}
	R(\phi) &= \begin{pmatrix}
		cos(\phi) & -\sin(\phi)\\
		\sin(\phi) & \cos(\phi)
	\end{pmatrix},
	\label{eq: rotationMat}\\
	R\left(\frac{\pi}{4}\right) &= \frac{1}{\sqrt{2}}\begin{pmatrix}
		1 & 1 \\ -1 & 1
	\end{pmatrix}.
\end{align}
\subsubsection*{b}
See equation (\ref{eq: rotationMat}).
\subsubsection*{c}
Right circularly polarized light is given by
\begin{equation}
	\ket{R} = \frac{1}{\sqrt{2}}\left( \ket{x}+i\ket{y} \right).
\end{equation}
\begin{equation}
	\phi(z,t) = \frac{1}{\sqrt{2}}e^{-i\omega t}\begin{pmatrix}
	e^{i k_x z} \\ e^{i k_y z}
	\end{pmatrix}.
\end{equation}
Thus,
\begin{equation}
	\ket{\psi} = \frac{1}{\sqrt{2}} \left( \ket{x} - i e^{i(k_x-k_y)Z}\ket{y} \right).
\end{equation}
\subsubsection*{d}
\begin{align}
	\rho_{\ket{R}} &= \op{R},\\
	&= \frac{1}{2} \left( \ket{x} + i\ket{y} \right)\left( \bra{x} - i\bra{y} \right),\\
	&= \frac{1}{2} \left( \hat{1} + \sigma_2 \right).
\end{align}
\subsubsection*{e}
\begin{equation}
	\rho_\psi = \frac{1}{2} \op{x} + \frac{1}{2} \op{y}.
\end{equation}
\subsection{}%2
\begin{align}
	\ev{R(\theta)}{x} &= \ev{(\cos\theta-i\sin\theta)}{x},\\
	&= \cos\theta - i\sin\theta\ev{\sigma_2}{x},\\
	&= \cos\theta.
\end{align}
\begin{align}
	\ev{R\left(\frac{\pi}{2}\right)}{x} &= 0,\\
	\ev{R\left(\pi\right)}{x} &= -1,\\
	\ev{R\left(2\pi\right)}{x} &= 1.
\end{align}
\subsection{}%3
\begin{align}
	&\ev{R_y(\theta)}{z,+}\\ &= \ev{\left(\cos\frac{\theta}{2}+i\sin\frac{\theta}{2}\right)}{z,+},\\
	&= \cos\frac{\theta}{2} + i\sin\frac{\theta}{2}\ev{\sigma_2}{z,+},\\
	&= \cos\frac{\theta}{2}.
\end{align}
\begin{align}
	\ev{R_y\left(\frac{\pi}{2}\right)}{z,+} &= \frac{1}{\sqrt{2}},\\
	\ev{R_y\left(\pi\right)}{z,+} &= 0,\\
	\ev{R_y\left(2\pi\right)}{z,+} &= -1.
\end{align}
\subsection{}%4
Let $U$ bet a unitary transformation.
Then
\[
	UU^\dagger = U^\dagger U = \hat{1}.
\]
Hence,
\[
	U^\dagger \hat{1} U = U^\dagger U \hat{1} = \mathbb{11} = \hat{1}.
\]
\subsection{}%5
\begin{equation}
	U^\dagger = \frac{1}{\sqrt{2}} (\hat{1}+i\sigma_3).
\end{equation}
\subsubsection*{a}
\begin{align}
	U\sigma_1U^\dagger &= \frac{1}{2}(\hat{1}-i\sigma_3)\sigma_1(\hat{1}+i\sigma_3),\\
	&= \frac{1}{2}(\sigma_1 - i\sigma_3\sigma_1)(\hat{1}+i\sigma_3),\\
	&= \frac{1}{2}(\sigma_1+i[\sigma_1,\sigma_3] - \sigma_1),\\
	&= \frac{1}{2} i (-2i\sigma_2),\\
	&= \sigma_2.
\end{align}
\subsubsection*{b}
\begin{align}
	U\ket{x,+} &= \frac{1}{2}(\hat{1}+i\sigma_3)(\ket{\uparrow}+\ket{\downarrow}),\\
	&= \frac{1}{2}(\ket{\uparrow}+\ket{\downarrow}-i\ket{\uparrow}+i\ket{\downarrow}),\\
	&= \frac{1}{\sqrt{2}}(\ket{\uparrow}+i\ket{\downarrow}).
	\label{eq: y eigenvec}
\end{align}
This expression (\ref{eq: y eigenvec}) is an eigenstate of $\sigma_2$.
\subsection{}%6
\begin{equation}
	U^\dagger = v_i^{(j)}.
\end{equation}
\subsubsection*{a}
\begin{align}
	UU^\dagger &= v_j^{*(i)}v_i^{(j)},\\
	&= \left\{\begin{array}{lr}
		1, & i=j \\
		0, & i\neq j
	\end{array}\right.,\\
	&= \hat{1}.
\end{align}
\subsubsection*{b}
\begin{align}
	U_{ij} v_i^{(n)} &= v_j^{*(i)}v_i^{(n)},\\
	&= \delta_{nj}\qq{(ortho.)}\\
	K' = UKU^\dagger:&\\
	K'U v^{(n)} &= UKU^\dagger U v^{(n)},\\
	&= UK v^{(n)},\\
	&= \lambda_n \left(Uv^{(n)}\right).
\end{align}
\subsection{}%7
\begin{equation}
	M = \begin{pmatrix}
	 1 & 0 & 0 \\
	 0 & 0 & 1 \\
	 0 & 1 & 0 \\
	\end{pmatrix}.
\end{equation}
\subsubsection*{a}
\begin{align}
	\left| \begin{matrix}
	 \lambda-1 & 0 & 0 \\
	 0 & \lambda & -1 \\
	 0 & -1 & \lambda
	\end{matrix}\right|\!\!\!\!\!\!\!\!\!\!\!\!&\nonumber\\
	&= (\lambda-1)(\lambda^2-1) = 0,\\
	\lambda &= 1,\pm i.
\end{align}
\subsubsection*{b}
\begin{align}
	\begin{pmatrix}
	 \lambda-1 & 0 & 0 \\
	 0 & \lambda & -1 \\
	 0 & -1 & \lambda
	\end{pmatrix}&
	\begin{pmatrix}
		a \\ b \\ c
	\end{pmatrix}
	= \begin{pmatrix}
		0 \\ 0 \\ 0
	\end{pmatrix}.\\
	a &= 0,\\
	c &= b\lambda.\\
	v_1 &= \frac{1}{\sqrt{2}}\begin{pmatrix}
		0 \\ 1 \\ 1
	\end{pmatrix},\\
	v_i &= \frac{1}{\sqrt{2}}\begin{pmatrix}
		0 \\ 1 \\ i
	\end{pmatrix},\\
	v_{-i} &= \frac{1}{\sqrt{2}}\begin{pmatrix}
		0 \\ 1 \\ -i
	\end{pmatrix}.
\end{align}
\subsection{}%8
\begin{equation}
	K = \begin{pmatrix}
		A & C^* \\
		C & B
	\end{pmatrix}.
\end{equation}
\subsubsection*{a}
\begin{align}
	& (\lambda - A)(\lambda-B)-C^*C = 0,\\
	& \lambda_\pm = \frac{A+B \pm \sqrt{(A^2-B^2)+4C^*C}}{2}.
\end{align}
\subsubsection*{b}
\begin{align}
	\begin{pmatrix}
		\lambda-A & -C^* \\
		-C & \lambda-B
	\end{pmatrix}
	& \begin{pmatrix}
		a \\ b
	\end{pmatrix}
	= \begin{pmatrix}
		0 \\ 0
	\end{pmatrix},\\
	a(\lambda-A) - bC^* &= 0,\\
	-aC+b(\lambda-B) &=0,\\
	a &= b \sqrt{\frac{C^*(\lambda-B)}{C(\lambda-A)}},
\end{align}
\begin{equation}
	v_\pm = \frac{1}{\sqrt{\frac{C^*(\lambda-B)}{C(\lambda-A}-1}}\begin{pmatrix}
		\sqrt{\frac{C^*(\lambda-B)}{C(\lambda-A}},\\
		1
	\end{pmatrix}
\end{equation}
\subsection{}%9
\begin{equation}
	\ket{\psi} = \frac{1}{2} (\sqrt{3} \ket{x} + \ket{y}).
\end{equation}
\begin{align}
	\ev{(E-\ev{E})^2}^{1/2} &= \sqrt{Np(1-p)},\\
	p &= \abs{\ip{x}{y}}^2 = \frac{3}{4},\\
	\ev{(E-\ev{E})^2}^{1/2} &= \frac{\sqrt{3N}}{4}.\\
	\ev{E} &= Np,\\
	&= \frac{3N}{4}.\\
	N &= \frac{10\mathrm{J}}{h\nu} \approx 3.32 \cdot 10^{19},\\
	\frac{\ev{(E-\ev{E})^2}^{1/2}}{\ev{E}} &= \frac{1}{\sqrt{3N}},\\
	&\approx 1.00 \cdot 10^{-10}\mathrm{J^{-1/2}}.
\end{align}

% \nocite{*}
% \printbibliography[title={References},heading=bibnumbered]


% \end{multicols*}
\end{document}
